theories/LambdaWP.v
@@ -381,9 +381,9 @@ Fixpoint wp (E:ctx) (t:trm) : formula :=
       wp_getval wp E t1 (fun v1 =>
         wp_getval wp E t2 (fun v2 =>
           wp_for_val v1 v2 (fun X => wp (Ctx.add x X E) t3)))
-  | trm_case t1 p t2 t3 => 
+  | trm_match t0 pts => wp_fail (* TODO
       wp_getval wp E t1 (fun v1 =>
-        wp_case_val v1 p (fun G => wp (Ctx.app G E) t2) (aux t3))
+        wp_case_val v1 p (fun G => wp (Ctx.app G E) t2) (aux t3)) *)
   | trm_fail => wp_fail
   end.
 
@@ -722,6 +722,7 @@ Proof using.
   intros v2. applys~ wp_sound_for_val.
 Qed.
 
+(*
 Lemma wp_sound_case_val : forall v1 p F2 F3 t2 t3 E,
   (forall (G:ctx), F2 G ===> wp_triple_ (Ctx.app G E) t2) ->
   F3 ===> wp_triple_ E t3 ->
@@ -747,6 +748,7 @@ Proof using.
   applys~ wp_sound_getval (fun t1 => trm_case t1 p t2 t3).
   intros v. applys~ wp_sound_case_val.
 Qed.
+*)
 
 Lemma wp_sound_constr : forall E id ts,
   (forall t, mem t ts -> wp_sound t) ->
@@ -782,7 +784,7 @@ Proof using.
   { applys* wp_sound_apps. }
   { applys* wp_sound_while. }
   { applys* wp_sound_for_trm. }
-  { applys* wp_sound_case_trm. }
+  { skip. (* applys* wp_sound_case_trm. *) }
   { applys wp_sound_fail. }
 Qed.
 
