theories/LambdaWPTactics.v
@@ -194,9 +194,9 @@ Ltac xwp_simpl :=
   LibList.combine 
   List.rev Datatypes.app List.fold_right List.map
   Wp WP_getval WP_getval_typed WP_getval_val WP_getval_int
-  WP_apps WP_apps_or_prim WP_constr WP_var
+  WP_apps WP_apps_or_prim WP_constr WP_var WP_match WP_case 
   hprop_forall_vars prop_forall_vars
-  trm_to_pat patvars patsubst combiner_to_trm
+  trm_case trm_to_pat patvars patsubst combiner_to_trm
   Ctx.app Ctx.empty Ctx.lookup Ctx.add 
   var_eq eq_var_dec 
   string_dec string_rec string_rect
